Add quickCode support for operand constructors (e.g. memory operands), and finish verification of Poly1305.vaf

tools/Vale/src/emit_common_base.fs
@@ -10,7 +10,6 @@ open System.Numerics
 
 let concise_lemmas = ref true;
 let precise_opaque = ref false;
-let fstar = ref false;
 let reprint_decls_rev = ref ([]:decls)
 let disable_verify = ref false
 let omit_unverified = ref false
